commit

player.lean
@@ -85,7 +85,7 @@ begin
   { exact d.f s₁ },
 end
 
-def Angel.modify_move {pw : ℕ} (a : Angel pw) (s : State)
+def Angel.set_move {pw : ℕ} (a : Angel pw) (s : State)
   (ma : Valid_angel_move pw s.board) : Angel pw :=
 begin
   refine ⟨λ s₁ h, _⟩, apply dite (s₁ = s); intro h₁,
@@ -93,7 +93,7 @@ begin
   { exact a.f s₁ h },
 end
 
-def Devil.modify_move {pw : ℕ} (d : Devil) (s : State)
+def Devil.set_move (d : Devil) (s : State)
   (md : Valid_devil_move s.board) : Devil :=
 begin
   refine ⟨λ s₁, _⟩, apply dite (s₁ = s); intro h₁,
