determinacy.lean
@@ -24,7 +24,69 @@ end
 
 -----
 
-lemma exi_angel_move_of_not_devil_hws {pw : ℕ} {s : State}
+lemma angel_hvm_of_not_devil_hws {pw : ℕ} {s : State}
+  (h : ¬devil_hws_at pw s) :
+  ∀ (md : Valid_devil_move s.board),
+  angel_has_valid_move pw (apply_devil_move s md.m).board :=
+begin
+  sorry
+end
+
+-- #exit
+
+lemma exi_moves_hws_of_not_devil_hws {pw : ℕ} {s : State}
+  (h : ¬devil_hws_at pw s) :
+  ∀ (md : Valid_devil_move s.board) (d : Devil),
+  ∃ (ma : Valid_angel_move pw (apply_devil_move s md.m).board) (a : Angel pw),
+  (init_game a d (apply_angel_move (apply_devil_move s md.m) ma.m)).angel_wins :=
+begin
+  rintro md d,
+  have h₁ := h,
+  change ¬∃ _, _ at h₁, push_neg at h₁,
+  let d₁ := d.set_move s md,
+  specialize h₁ d₁,
+  cases h₁ with a h₁,
+  let s' : State := apply_devil_move s md.m,
+  change apply_devil_move s md.m with s',
+  use [a.f s' (angel_hvm_of_not_devil_hws h md), a],
+  generalize_proofs h₂,
+  change apply_devil_move s md.m with s' at h₂,
+  rw not_devil_wins_at at h₁,
+  convert angel_wins_at_play_move_of h₁,
+  rw init_game_play_move,
+  ext,
+  {
+    symmetry,
+    exact play_move_at_players_eq'.1,
+  },
+  {
+    symmetry,
+    -- exact play_move_at_players_eq'.2,
+    sorry
+  },
+  {
+    sorry,
+  },
+  {
+    apply (true_iff _).mpr,
+    rw play_angel_move_at,
+    have h₃ : (play_devil_move_at (init_game a d s)).s = s',
+    {
+      rw play_devil_move_at,
+      change apply_devil_move s (d.f s).m = s',
+      rw apply_devil_move,
+      sorry
+    },
+    simp_rw h₃,
+    sorry
+    -- rw dif_pos h₂,
+    -- triv,
+  },
+end
+
+#exit
+
+lemma exi_angel_move_hws_of_not_devil_hws {pw : ℕ} {s : State}
   (h : ¬devil_hws_at pw s) :
   ∀ (md : Valid_devil_move s.board),
   ∃ (ma : Valid_angel_move pw (apply_devil_move s md.m).board),
@@ -41,7 +103,7 @@ begin
   { refine (_ : ∃ (ma : Valid_angel_move pw s'.board),
       ¬devil_hws_at pw (apply_angel_move s' ma.m)).some,
     rcases h₁ with ⟨s, md, h₁, rfl⟩,
-    use (exi_angel_move_of_not_devil_hws h₁ _).some,
+    use (exi_angel_move_hws_of_not_devil_hws h₁ _).some,
     generalize_proofs h₂, exact h₂.some_spec },
   { exact ⟨_, h.some_spec⟩ },
 end
@@ -61,7 +123,7 @@ begin
   let s' := apply_devil_move s md.m,
   have h₃ : ∃ (ma : Valid_angel_move pw s'.board),
     ¬devil_hws_at pw (apply_angel_move s' ma.m),
-  { exact exi_angel_move_of_not_devil_hws ih md },
+  { exact exi_angel_move_hws_of_not_devil_hws ih md },
   have ma := h₃.some, have h₄ := h₃.some_spec,
   convert h₄, change Game.s (dite _ _ _) = _,
   have h₅ : angel_has_valid_move pw s'.board := ⟨_, ma.h⟩,
@@ -85,7 +147,7 @@ begin
     congr, symmetry, exact play_at_players_eq.2 },
   rw h₁, clear h₁, have h₁ : angel_has_valid_move pw s'.board,
   { have h₁ : ¬devil_hws_at pw s := not_devil_hws_at_play_of_not_devil_hws rfl h,
-    exact ⟨_, (exi_angel_move_of_not_devil_hws h₁ md).some.h⟩ },
+    exact ⟨_, (exi_angel_move_hws_of_not_devil_hws h₁ md).some.h⟩ },
   change Game.act (dite _ _ _), change (g.set_state s').s with s',
   rw dif_pos h₁, exact ih,
 end
